x86/ConstpropOpproofSSA.v
@@ -1,0 +1,177 @@
+(* *********************************************************************)
+(*                                                                     *)
+(*              The Compcert verified compiler                         *)
+(*                                                                     *)
+(*          Xavier Leroy, INRIA Paris-Rocquencourt                     *)
+(*                                                                     *)
+(*  Copyright Institut National de Recherche en Informatique et en     *)
+(*  Automatique.  All rights reserved.  This file is distributed       *)
+(*  under the terms of the INRIA Non-Commercial License Agreement.     *)
+(*                                                                     *)
+(* *********************************************************************)
+
+(** Correctness proof for simple sparse constant propagation (processor-dependent part). *)
+
+Require Import Coqlib.
+Require Import Integers.
+Require Import Floats.
+Require Import Values.
+Require Import Memory.
+Require Import Globalenvs.
+Require Import Events.
+Require Import Op.
+Require Import SSAtool.
+Require Import ConstpropOp.
+
+(** * Correctness of the static analysis *)
+(* DD: Diff to ConstpropOpproof : the type of genv... *)
+
+Section ANALYSIS.
+
+Variable ge: genv.
+Variable sp: val.
+
+(** We first show that the dataflow analysis is correct with respect
+  to the dynamic semantics: the approximations (sets of values) 
+  of a register at a program point predicted by the static analysis
+  are a superset of the values actually encountered during concrete
+  executions.  We formalize this correspondence between run-time values and
+  compile-time approximations by the following predicate. *)
+
+Definition val_match_approx (a: approx) (v: val) : Prop :=
+  match a with
+  | Unknown => True
+  | I p => v = Vint p
+  | F p => v = Vfloat p
+  | L p => v = Vlong p
+  | G symb ofs => v = symbol_address ge symb ofs
+  | S ofs => v = Val.add sp (Vint ofs)
+  | Novalue => False
+  end.
+
+Inductive val_list_match_approx: list approx -> list val -> Prop :=
+  | vlma_nil:
+      val_list_match_approx nil nil
+  | vlma_cons:
+      forall a al v vl,
+      val_match_approx a v ->
+      val_list_match_approx al vl ->
+      val_list_match_approx (a :: al) (v :: vl).
+
+Ltac SimplVMA :=
+  match goal with
+  | H: (val_match_approx (I _) ?v) |- _ =>
+      simpl in H; (try subst v); SimplVMA
+  | H: (val_match_approx (F _) ?v) |- _ =>
+      simpl in H; (try subst v); SimplVMA
+  | H: (val_match_approx (L _) ?v) |- _ =>
+      simpl in H; (try subst v); SimplVMA
+  | H: (val_match_approx (G _ _) ?v) |- _ =>
+      simpl in H; (try subst v); SimplVMA
+  | H: (val_match_approx (S _) ?v) |- _ =>
+      simpl in H; (try subst v); SimplVMA
+  | _ =>
+      idtac
+  end.
+
+Ltac InvVLMA :=
+  match goal with
+  | H: (val_list_match_approx nil ?vl) |- _ =>
+      inv H
+  | H: (val_list_match_approx (?a :: ?al) ?vl) |- _ =>
+      inv H; SimplVMA; InvVLMA
+  | _ =>
+      idtac
+  end.
+
+(** We then show that [eval_static_operation] is a correct abstract
+  interpretations of [eval_operation]: if the concrete arguments match
+  the given approximations, the concrete results match the
+  approximations returned by [eval_static_operation]. *)
+
+Lemma eval_static_condition_correct:
+  forall cond al vl m b,
+  val_list_match_approx al vl ->
+  eval_static_condition cond al = Some b ->
+  eval_condition cond vl m = Some b.
+Proof.
+  intros until b.
+  unfold eval_static_condition. 
+  case (eval_static_condition_match cond al); intros;
+  InvVLMA; simpl; congruence.
+Qed.
+
+Remark shift_symbol_address:
+  forall symb ofs n,
+  symbol_address ge symb (Int.add ofs n) = Val.add (symbol_address ge symb ofs) (Vint n).
+Proof.
+  unfold symbol_address; intros. destruct (Genv.find_symbol ge symb); auto. 
+Qed.
+
+Lemma eval_static_addressing_correct:
+  forall addr al vl v,
+  val_list_match_approx al vl ->
+  eval_addressing ge sp addr vl = Some v ->
+  val_match_approx (eval_static_addressing addr al) v.
+Proof.
+  intros until v. unfold eval_static_addressing.
+  case (eval_static_addressing_match addr al); intros;
+  InvVLMA; simpl in *; FuncInv; try subst v; auto.
+  rewrite shift_symbol_address; auto.
+  rewrite Val.add_assoc. auto.
+  repeat rewrite shift_symbol_address. auto.
+  fold (Val.add (Vint n1) (symbol_address ge id ofs)).
+  repeat rewrite shift_symbol_address. repeat rewrite Val.add_assoc. rewrite Val.add_permut. auto.
+  repeat rewrite Val.add_assoc. decEq; simpl. rewrite Int.add_assoc. auto.
+  fold (Val.add (Vint n1) (Val.add sp (Vint ofs))).
+  rewrite Val.add_assoc. rewrite Val.add_permut. rewrite Val.add_assoc. 
+  simpl. rewrite Int.add_assoc; auto.
+  rewrite shift_symbol_address. auto.
+  rewrite Val.add_assoc. auto. 
+  rewrite shift_symbol_address. auto.
+  rewrite shift_symbol_address. rewrite Int.mul_commut; auto. 
+Qed.
+
+Lemma eval_static_operation_correct:
+  forall op al vl m v,
+  val_list_match_approx al vl ->
+  eval_operation ge sp op vl m = Some v ->
+  val_match_approx (eval_static_operation op al) v.
+Proof.
+  intros until v.
+  unfold eval_static_operation. 
+  case (eval_static_operation_match op al); intros;
+  InvVLMA; simpl in *; FuncInv; try subst v; auto.
+  destruct (propagate_float_constants tt); simpl; auto.
+  rewrite Int.sub_add_opp. rewrite shift_symbol_address. rewrite Val.sub_add_opp. auto.
+  destruct (Int.eq n2 Int.zero). inv H0. 
+    destruct (Int.eq n1 (Int.repr Int.min_signed) && Int.eq n2 Int.mone); inv H0; simpl; auto.
+  destruct (Int.eq n2 Int.zero); inv H0; simpl; auto.
+  destruct (Int.eq n2 Int.zero). inv H0. 
+    destruct (Int.eq n1 (Int.repr Int.min_signed) && Int.eq n2 Int.mone); inv H0; simpl; auto.
+  destruct (Int.eq n2 Int.zero); inv H0; simpl; auto.
+  destruct (Int.ltu n2 Int.iwordsize); simpl; auto.
+  destruct (Int.ltu n Int.iwordsize); simpl; auto.
+  destruct (Int.ltu n2 Int.iwordsize); simpl; auto.
+  destruct (Int.ltu n Int.iwordsize); simpl; auto.
+  destruct (Int.ltu n (Int.repr 31)); inv H0. simpl; auto.
+  destruct (Int.ltu n2 Int.iwordsize); simpl; auto.
+  destruct (Int.ltu n Int.iwordsize); simpl; auto.
+  destruct (Int.ltu n Int.iwordsize); simpl; auto.
+  destruct (Int.ltu n Int.iwordsize);
+  destruct (Int.ltu (Int.sub Int.iwordsize n) Int.iwordsize); simpl; auto.
+  eapply eval_static_addressing_correct; eauto.
+  unfold eval_static_intoffloat.
+  destruct (Float.intoffloat n1) eqn:?; simpl in H0; inv H0.
+  simpl; auto.
+  destruct (propagate_float_constants tt); simpl; auto.
+  unfold eval_static_condition_val. destruct (eval_static_condition c vl0) as [b|] eqn:?.
+  rewrite (eval_static_condition_correct _ _ _ m _ H Heqo). 
+  destruct b; simpl; auto.
+  simpl; auto.
+Qed.
+
+(*
+(** * Correctness of strength reduction *)
+*)
+End ANALYSIS.
